GrammarAnalysis.v
@@ -1,0 +1,163 @@
+Require Import List MSets.
+Require Import GallStar.LLPrediction_complete.
+Require Import GallStar.Utils.
+Import ListNotations.
+
+Module GrammarAnalysisFn (Import D : Defs.T).
+
+  Module Export LLPC := LLPredictionCompleteFn D.
+
+  Definition edge := (suffix_frame * suffix_frame)%type.
+
+  Lemma edge_eq_dec :
+    forall e e' : edge, {e = e'} + {e <> e'}.
+  Proof.
+    repeat decide equality; try apply t_eq_dec; try apply nt_eq_dec.
+  Qed.
+
+  Module MDT_Edge.
+    Definition t      := edge.
+    Definition eq_dec := edge_eq_dec.
+  End MDT_Edge.
+  Module Edge_as_DT   := Make_UDT(MDT_Edge).
+  Module EdgeSet      := MSetWeakList.Make Edge_as_DT.
+  Module EdgeSetFacts := WFactsOn Edge_as_DT EdgeSet.
+  Module ES           := EdgeSet.
+
+  Definition setOf (es : list edge) : ES.t :=
+    fold_right ES.add ES.empty es.
+
+  Definition bin (e : edge) (es : list edge) : bool :=
+    if in_dec edge_eq_dec e es then true else false.
+
+  Definition src (e : edge) : suffix_frame := fst e.
+  Definition dst (e : edge) : suffix_frame := snd e.
+
+  Fixpoint pushEdges' (g : grammar) (x : nonterminal) (ys : list symbol) : list edge :=
+    match ys with 
+    | []          => []
+    | T _ :: ys'  => pushEdges' g x ys'
+    | NT y :: ys' =>
+      let es := map (fun rhs => (SF (Some x) ys, SF (Some y) rhs))
+                    (rhssForNt g y)
+      in  es ++ pushEdges' g x ys'
+    end.
+
+  Definition pushEdges (g : grammar) : list edge :=
+    flat_map (fun p => pushEdges' g (lhs p) (rhs p)) g.
+
+  Fixpoint returnEdges' (x : nonterminal) (ys : list symbol) : list edge :=
+    match ys with
+    | []          => []
+    | T _ :: ys'  => returnEdges' x ys'
+    | NT y :: ys' =>
+      (SF (Some y) [], SF (Some x) ys') :: returnEdges' x ys'
+    end.
+
+  Definition returnEdges (g : grammar) : list edge :=
+    flat_map (fun p => returnEdges' (lhs p) (rhs p)) g.
+
+  Definition finalReturnEdges g : list edge :=
+    map (fun x => (SF (Some x) [], SF None [])) (lhss g).
+
+  Definition epsilonEdges g : list edge :=
+    pushEdges g ++ returnEdges g ++ finalReturnEdges g.
+
+  Fixpoint dsts (es : list edge) (s : suffix_frame) : list suffix_frame :=
+    match es with
+    | []             => []
+    | (s', d) :: es' =>
+      if suffix_frame_eq_dec s' s then d :: dsts es' s else dsts es' s
+    end.
+
+  Definition newEdges' (es : list edge) (e : edge) : list edge :=
+    let (a, b) := e in
+    let cs     := filter (fun c => negb (bin (a, c) es)) (dsts es b)
+    in  oneToMany a cs.
+
+  Definition newEdges (es : list edge) : list edge :=
+    flat_map (newEdges' es) es.
+
+  Definition allSrcs es : list suffix_frame := map src es.
+  Definition allDsts es : list suffix_frame := map dst es.
+
+  Definition allEdges es : list edge := 
+    let ss := allSrcs es in
+    let ds := allDsts es in
+    flat_map (fun s => oneToMany s ds) ss.
+
+  Definition stable (fr : suffix_frame) : bool :=
+    match fr with
+    | SF None []             => true
+    | SF (Some x) (T _ :: _) => true
+    | _                      => false
+    end.
+
+  Fixpoint stablePositions' x ys : list suffix_frame :=
+    match ys with
+    | []          => []
+    | T a :: ys'  => SF (Some x) ys :: stablePositions' x ys'
+    | NT _ :: ys' => stablePositions' x ys'
+    end.
+
+  Definition stablePositions (g : grammar) : list suffix_frame :=
+    SF None [] :: flat_map (fun p => stablePositions' (lhs p) (rhs p)) g.
+
+  (* might not be necessary *)
+  Definition reflEdges (g : grammar) : list edge :=
+    map (fun p => (p, p)) (stablePositions g).
+
+  Definition m (es : list edge) : nat :=
+    ES.cardinal (ES.diff (setOf (allEdges es)) (setOf es)).
+
+  Axiom magic : forall A, A.
+
+  Program Fixpoint transClosure (es : list edge)
+          { measure (m es) } : list edge :=
+    let es' := newEdges es in
+    match es' as es'' return es' = es'' -> _ with
+    | []     => fun _   => es
+    | _ :: _ => fun heq => transClosure (es' ++ es)
+    end eq_refl.
+  Next Obligation.
+    rewrite heq; simpl.
+    unfold m.
+    apply magic.
+  Defined.
+
+  Definition dstStable (e : edge) : bool :=
+    let (_, b) := e in stable b.
+
+  Definition stableEdges (es : list edge) : list edge :=
+    filter dstStable es.
+
+  (* Maybe we don't need the refl edges *)
+  Definition mkGraphEdges (g : grammar) : list edge :=
+    stableEdges (transClosure (epsilonEdges g)) ++ (reflEdges g).
+
+  (* A closure graph is a map where each key K is a suffix frame 
+     (i.e., grammar location), and each value V is a list of frames 
+     that are epsilon-reachable from K *)
+  (* Maybe the value should be a set *)
+  Definition closure_map := FM.t (list suffix_frame).
+
+  Definition addEdge (e : edge) (m : closure_map) : closure_map :=
+    let (k, v) := e in
+    match FM.find k m with
+    | Some vs => FM.add k (v :: vs) m
+    | None    => FM.add k [v] m
+    end.
+
+  Definition fromEdges (es : list edge) : closure_map :=
+    fold_right addEdge (FM.empty (list suffix_frame)) es.
+
+  Definition mkClosureMap (g : grammar) : closure_map :=
+    fromEdges (mkGraphEdges g).
+
+  Definition destFrames (cm : closure_map) (fr : suffix_frame) : list suffix_frame :=
+    match FM.find fr cm with
+    | Some frs => frs
+    | None     => []
+    end.
+
+End GrammarAnalysisFn.
